src/SoftBound/sb_ns_ds.v
@@ -1,0 +1,643 @@
+Add LoadPath "../ssa/ott".
+Add LoadPath "../ssa/monads".
+Add LoadPath "../ssa".
+Add LoadPath "../ssa/compcert".
+Add LoadPath "../../../theory/metatheory_8.3".
+Add LoadPath "../TV".
+Require Import ssa_def.
+Require Import ssa_lib.
+Require Import ssa_dynamic.
+Require Import trace.
+Require Import Memory.
+Require Import genericvalues.
+Require Import alist.
+Require Import Integers.
+Require Import Values.
+Require Import Coqlib.
+Require Import monad.
+Require Import Metatheory.
+Require Import Znumtheory.
+Require Import sb_ds_def.
+Require Import sb_ns_def.
+Require Import ndopsem_dsop.
+
+Export SBnsop.
+Export SBopsem.
+
+Definition instantiate_EC (ec1 : SBopsem.ExecutionContext) 
+  (ec2 : SBnsop.ExecutionContext) : Prop :=
+match ec1, ec2 with
+| SBopsem.mkEC f1 b1 cs1 tmn1 lc1 rm1 als1, 
+  SBnsop.mkEC f2 b2 cs2 tmn2 lc2 rm2 als2 =>
+    f1 = f2 /\ b1 = b2 /\ cs1 = cs2 /\ tmn1 = tmn2 /\
+    instantiate_locals lc1 lc2 /\ rm1 = rm2 /\ als1 = als2
+end.
+
+Fixpoint instantiate_ECs (ecs1 : SBopsem.ECStack) (ecs2 : SBnsop.ECStack) 
+  : Prop :=
+match ecs1, ecs2 with
+| nil, nil => True
+| ec1::ecs1', ec2::ecs2' => instantiate_EC ec1 ec2 /\ instantiate_ECs ecs1' ecs2'
+| _, _ => False
+end.
+
+Definition instantiate_State (st1 : SBopsem.State) (st2 : SBnsop.State) 
+  : Prop :=
+match st1, st2 with
+| SBopsem.mkState s1 td1 ps1 ecs1 gl1 fs1 M1 MM1,
+  SBnsop.mkState s2 td2 ps2 ecs2 gl2 fs2 M2 MM2 =>
+    s1 = s2 /\ td1 = td2 /\ ps1 = ps2 /\ instantiate_ECs ecs1 ecs2 /\ gl1 = gl2
+    /\ fs1 = fs2 /\ M1 = M2 /\ MM1 = MM2
+end.
+
+Lemma instantiate_locals__returnResult : forall TD rt Result lc1 lc2 gl gv1 rm 
+    md,
+  instantiate_locals lc1 lc2 -> 
+  SBopsem.returnResult TD rt Result lc1 rm gl = Some (gv1, md) ->
+  exists gv2, 
+    SBnsop.returnResult TD rt Result lc2 rm gl = Some (gv2, md) /\
+    instantiate_gv gv1 gv2.
+Proof.
+  intros.  
+  unfold SBopsem.returnResult in H0.
+  remember (getOperandValue TD Result lc1 gl) as R.
+  destruct R; tinv H0.
+  symmetry in HeqR.
+  eapply instantiate_locals__getOperandValue in HeqR; eauto.
+  destruct HeqR as [gvs2 [J1 J2]].
+  unfold SBnsop.returnResult.
+  rewrite J1. 
+  destruct (isPointerTypB rt); inv H0; eauto.
+  destruct (get_reg_metadata TD gl rm Result); inv H2.
+  exists gvs2. split; auto using instantiate_locals__updateAddAL.
+Qed.
+
+Lemma instantiate_locals__returnUpdateLocals : forall TD lc1 lc2 lc1' lc2' Result
+    gl lc1'' c rm rm' rt rm'',
+  instantiate_locals lc1 lc2 -> 
+  instantiate_locals lc1' lc2' -> 
+  SBopsem.returnUpdateLocals TD c rt Result lc1 lc1' rm rm' gl = 
+    ret (lc1'',rm'') ->
+  exists lc2'', 
+    SBnsop.returnUpdateLocals TD c rt Result lc2 lc2' rm rm' gl = 
+      ret (lc2'',rm'') /\
+    instantiate_locals lc1'' lc2''. 
+Proof.
+  intros.
+  unfold SBopsem.returnUpdateLocals in H1.
+  remember (returnResult TD rt Result lc1 rm gl) as R.
+  destruct R as [[gr md]|]; tinv H1.
+  symmetry in HeqR.
+  eapply instantiate_locals__returnResult in HeqR; eauto.
+  destruct HeqR as [gvs2 [J1 J2]].
+  unfold SBnsop.returnUpdateLocals.
+  rewrite J1. 
+  destruct c; inv H1; eauto.
+  destruct n; inv H3.
+    exists lc2'. split; auto.
+    destruct (SBopsem.isReturnPointerTypB t); inv H2.
+      exists (updateAddAL GVs lc2' i0 gvs2).   
+      split; auto using instantiate_locals__updateAddAL.
+
+      exists (updateAddAL GVs lc2' i0 gvs2).   
+      split; auto using instantiate_locals__updateAddAL.
+Qed.
+
+Fixpoint instantiate_localms (lcm1 : list (id*GenericValue*option metadata)) 
+  (lcm2 : list (id*GVs*option metadata)) : Prop :=
+match lcm1, lcm2 with
+| nil, nil => True
+| (id1,gv1,omd1)::lcm1', (id2,gvs2,omd2)::lcm2' => 
+    id1=id2 /\ instantiate_gv gv1 gvs2 /\ instantiate_localms lcm1' lcm2' /\ 
+    omd1 = omd2
+| _, _ => False
+end.
+
+Lemma instantiate_locals__getIncomingValuesForBlockFromPHINodes : forall TD b
+    gl lc1 lc2 (Hlc : instantiate_locals lc1 lc2) ps re1 rm,  
+  SBopsem.getIncomingValuesForBlockFromPHINodes TD ps b gl lc1 rm = Some re1 ->
+  exists re2,
+    SBnsop.getIncomingValuesForBlockFromPHINodes TD ps b gl lc2 rm = Some re2 /\
+    instantiate_localms re1 re2.
+Proof.
+  induction ps; simpl; intros.  
+    inv H. exists nil. simpl. auto.
+
+    destruct a.
+    destruct (getValueViaBlockFromValuels l0 b); tinv H.
+    remember (getOperandValue TD v lc1 gl) as R.
+    destruct R; tinv H.
+    symmetry in HeqR.  
+    eapply instantiate_locals__getOperandValue in HeqR; eauto.
+    destruct HeqR as [gvs2 [J1 J2]].
+    remember (getIncomingValuesForBlockFromPHINodes TD ps b gl lc1 rm) as R1.
+    destruct R1; inv H.  
+    rewrite J1.
+    symmetry in HeqR1.
+    destruct (@IHps l1 rm) as [re2 [J3 J4]]; auto.
+    rewrite J3. 
+    destruct (isPointerTypB t); inv H1.
+      destruct (get_reg_metadata TD gl rm v); inv H0.
+      exists ((i0, gvs2, ret m) :: re2). simpl. auto.
+
+      exists ((i0, gvs2, merror) :: re2). simpl. auto.
+Qed.
+
+Lemma instantiate_locals__updateValuesForNewBlock : forall lc1 lc2 re1 re2 rm 
+    lc1' rm',
+  instantiate_locals lc1 lc2 ->
+  instantiate_localms re1 re2 ->
+  SBopsem.updateValuesForNewBlock re1 lc1 rm = (lc1', rm') ->
+  exists lc2', 
+    SBnsop.updateValuesForNewBlock re2 lc2 rm = (lc2', rm') /\
+    instantiate_locals lc1' lc2'.
+Proof.
+  induction re1; destruct re2; simpl; intros; auto.
+    inv H1. eauto.
+    inv H0.
+    destruct a. destruct p. inv H0.
+
+    destruct a. destruct p0. destruct p. destruct p.
+    destruct H0 as [eq [J1 [J2 eq']]]; subst.
+    remember (updateValuesForNewBlock re1 lc1 rm) as R.
+    destruct R as [lc' rm''].
+    symmetry in HeqR. eapply IHre1 in HeqR; eauto.
+    destruct HeqR as [lc2' [J3 J4]].
+    rewrite J3.
+    destruct o0; inv H1.
+      exists (updateAddAL _ lc2' i1 g0). 
+      split; auto using instantiate_locals__updateAddAL.
+
+      exists (updateAddAL _ lc2' i1 g0). 
+      split; auto using instantiate_locals__updateAddAL.
+Qed.
+
+Lemma instantiate_locals__switchToNewBasicBlock : forall TD lc1 lc2 gl lc1' b b'
+    rm rm',
+  instantiate_locals lc1 lc2 -> 
+  SBopsem.switchToNewBasicBlock TD b' b gl lc1 rm = Some (lc1',rm') ->
+  exists lc2', SBnsop.switchToNewBasicBlock TD b' b gl lc2 rm = Some (lc2',rm') 
+    /\ instantiate_locals lc1' lc2'. 
+Proof.
+  intros.
+  unfold switchToNewBasicBlock in H0.
+  unfold SBnsop.switchToNewBasicBlock.
+  remember (getIncomingValuesForBlockFromPHINodes TD (getPHINodesFromBlock b') b
+           gl lc1 rm) as R.
+  destruct R; inv H0.
+  symmetry in HeqR.
+  eapply instantiate_locals__getIncomingValuesForBlockFromPHINodes in HeqR; eauto.
+  destruct HeqR as [re2 [J1 J2]].
+  rewrite J1.
+  eapply instantiate_locals__updateValuesForNewBlock in H2; eauto.
+  destruct H2 as [lc2' [J3 J4]].
+  rewrite J3. eauto.
+Qed.
+
+Fixpoint instantiate_gvms (l1 : list (GenericValue * option metadata)) 
+  (l2 : list (GVs * option metadata)) :=
+match l1, l2 with
+| nil, nil => True
+| (gv1,omd1)::l1', (gvs2,omd2)::l2' => 
+    instantiate_gv gv1 gvs2 /\ omd1 = omd2 /\ instantiate_gvms l1' l2'
+| _, _ => False
+end.
+
+Lemma instantiate_locals__params2GVs : forall TD lc1 lc2 gl rm
+  (Hlc:instantiate_locals lc1 lc2) lp gvms1,
+  SBopsem.params2GVs TD lp lc1 gl rm = Some gvms1 ->
+  exists gvsms2, SBnsop.params2GVs TD lp lc2 gl rm = Some gvsms2 /\
+    instantiate_gvms gvms1 gvsms2.
+Proof.
+  induction lp; simpl; intros.
+    inv H. exists nil. simpl. auto.
+
+    destruct a.
+    remember (getOperandValue TD v lc1 gl) as R1.
+    destruct R1; tinv H.
+    remember (params2GVs TD lp lc1 gl rm) as R2.
+    destruct R2; tinv H.
+    inv H.
+    symmetry in HeqR1.
+    eapply instantiate_locals__getOperandValue in HeqR1; eauto.
+    destruct HeqR1 as [gvs2 [H3 H4]].
+    destruct (@IHlp l0) as [gvsss2 [J1 J2]]; auto.
+    rewrite H3. rewrite J1. 
+    destruct (isPointerTypB t); inv H1.
+      exists ((gvs2, get_reg_metadata TD gl rm v) :: gvsss2). simpl. split; auto.
+      exists ((gvs2, merror) :: gvsss2). simpl. split; auto.
+Qed.
+
+Lemma instantiate_locals__initializeFrameValues : forall lc1 lc2 rm
+  (H2: instantiate_locals lc1 lc2) la gvs1 gvs2 lc1' rm'
+  (H1 : instantiate_gvms gvs1 gvs2),
+  _initializeFrameValues la gvs1 lc1 rm = (lc1', rm') ->
+  exists lc2', 
+    SBnsop._initializeFrameValues la gvs2 lc2 rm = (lc2', rm') /\
+    instantiate_locals lc1' lc2'.
+Proof.
+  induction la; simpl; intros; auto.
+    inv H. eauto.
+
+    destruct a. destruct p.
+    destruct gvs1; simpl.
+      remember (_initializeFrameValues la nil lc1 rm) as R.
+      destruct R as [lc1'' rm''].
+      destruct gvs2; inv H1.
+      symmetry in HeqR.
+      apply IHla with (gvs2:=nil) in HeqR; simpl; eauto.
+      destruct HeqR as [lc2' [J1 J2]].
+      rewrite J1.
+      destruct (isPointerTypB t); inv H.
+        unfold SBnsop.prop_reg_metadata.
+        exists (updateAddAL GVs lc2' i0 ($ gundef t # t $)). 
+        split; auto.
+          apply instantiate_locals__updateAddAL; 
+            auto using instantiate_gv__gv2gvs. 
+
+        exists (updateAddAL GVs lc2' i0 ($ gundef t # t $)). 
+        split; auto.
+          apply instantiate_locals__updateAddAL; 
+            auto using instantiate_gv__gv2gvs. 
+
+      destruct p.
+      simpl in H1.
+      destruct gvs2; tinv H1. 
+      destruct p. destruct H1 as [J1 [J2 J3]]; subst.
+      remember (_initializeFrameValues la gvs1 lc1 rm) as R.
+      destruct R as [lc1'' rm''].
+      symmetry in HeqR.
+      eapply IHla in HeqR; simpl; eauto.
+      destruct HeqR as [lc2' [J1' J2']].
+      rewrite J1'.
+      unfold SBnsop.prop_reg_metadata.
+      destruct (isPointerTypB t); inv H.
+        destruct o0; inv H1.
+          exists (updateAddAL GVs lc2' i0 g0). 
+          split; auto using instantiate_locals__updateAddAL.
+
+          exists (updateAddAL GVs lc2' i0 g0). 
+          split; auto using instantiate_locals__updateAddAL.
+        exists (updateAddAL GVs lc2' i0 g0). 
+        split; auto using instantiate_locals__updateAddAL.
+Qed.           
+
+Lemma instantiate_locals__initLocals : forall gvs1 gvss2 lc1 rm
+  (H : instantiate_gvms gvs1 gvss2) la,
+  initLocals la gvs1 = (lc1, rm) ->
+  exists lc2, 
+    SBnsop.initLocals la gvss2 = (lc2, rm) /\ instantiate_locals lc1 lc2.
+Proof.
+  unfold initLocals, SBnsop.initLocals.
+  intros.
+  eapply instantiate_locals__initializeFrameValues; eauto.
+    simpl. auto.
+Qed.
+
+Lemma instantiate_locals__exCallUpdateLocals : forall lc1 lc2 lc1' rid oResult 
+    nr ft rm rm',
+  instantiate_locals lc1 lc2 -> 
+  SBopsem.exCallUpdateLocals ft nr rid oResult lc1 rm = ret (lc1',rm') ->
+  exists lc2', 
+    SBnsop.exCallUpdateLocals ft nr rid oResult lc2 rm = ret (lc2',rm') /\
+    instantiate_locals lc1' lc2'. 
+Proof.
+  intros.
+  unfold SBopsem.exCallUpdateLocals in H0.
+  unfold SBnsop.exCallUpdateLocals.
+  destruct nr; inv H0; eauto.
+  destruct oResult; inv H2; eauto.
+  destruct ft; inv H1; 
+    eauto using instantiate_locals__updateAddAL, instantiate_gv__gv2gvs.
+  destruct ft; inv H2; 
+    eauto using instantiate_locals__updateAddAL, instantiate_gv__gv2gvs.
+Qed.
+
+Ltac simpl_nd_sbds :=
+  match goal with
+  | [Hsim : instantiate_State {| ECS := _::_::_ |} ?st2 |- _ ] =>
+     destruct st2 as [S' TD' Ps' ECs' gl' fs' M' MM'];
+     destruct Hsim as [eq1 [eq2 [eq3 [Hsim [eq4 [eq5 [eq6 eq7]]]]]]]; subst;
+     destruct ECs' as [|[f1' b1' cs1' tmn1' lc1' rm1' als1'] ECs']; 
+       try solve [inversion Hsim];
+     simpl in Hsim; destruct Hsim as [Hsim1 Hsim2];
+     destruct ECs' as [|[f2' b2' cs2' tmn2' lc2' rm2' als2'] ECs'];
+       try solve [inversion Hsim2];
+     destruct Hsim2 as [Hsim2 Hsim3];
+     destruct Hsim1 as [J1 [J2 [J3 [J4 [Hsim1 [J6 J7]]]]]]; subst;
+     destruct Hsim2 as [J1 [J2 [J3 [J4 [Hsim2 [J6 J7]]]]]]; subst
+  | [Hsim : instantiate_State {| ECS := _::_|} ?st2 |- _ ] =>
+     destruct st2 as [S' TD' Ps' ECs' gl' fs' M' MM'];
+     destruct Hsim as [eq1 [eq2 [eq3 [Hsim [eq4 [eq5 [eq6 eq7]]]]]]]; subst;
+     destruct ECs' as [|[f1' b1' cs1' tmn1' lc1' rm1' als1'] ECs']; 
+       try solve [inversion Hsim];
+     simpl in Hsim; destruct Hsim as [Hsim1 Hsim2];
+     destruct Hsim1 as [J1 [J2 [J3 [J4 [Hsim1 [J6 J7]]]]]]; subst
+  end.
+
+Hint Constructors SBnsop.nsInsn.
+
+Lemma instantiate_dsInsn : forall st1 st2 st1' tr,
+  instantiate_State st1 st2 ->
+  SBopsem.dsInsn st1 st1' tr ->
+  (exists st2', SBnsop.nsInsn st2 st2' tr /\ instantiate_State st1' st2').
+Proof.
+  intros st1 st2 st1' tr Hsim Hop.  
+  (sb_dsInsn_cases (induction Hop) Case).
+Case "dsReturn". simpl_nd_sbds. 
+  eapply instantiate_locals__returnUpdateLocals in H1; eauto.
+  destruct H1 as [lc2'' [H1 H2]].
+  exists (SBnsop.mkState S' TD' Ps' 
+    ((SBnsop.mkEC f2' b2' cs' tmn2' lc2'' rm'' als2')::ECs') gl' fs' Mem' MM').
+  split; eauto.
+    repeat (split; auto).
+Case "dsReturnVoid". simpl_nd_sbds. 
+  exists (SBnsop.mkState S' TD' Ps' 
+    ((SBnsop.mkEC f2' b2' cs' tmn2' lc2' rm2' als2')::ECs') gl' fs' Mem' MM').
+  split; eauto.
+    repeat (split; auto).
+Case "dsBranch". simpl_nd_sbds. 
+  eapply instantiate_locals__switchToNewBasicBlock in H1; eauto.
+  eapply instantiate_locals__getOperandValue in H; eauto.
+  destruct H as [gvs2 [J1 J2]].
+  destruct H1 as [lc2' [J3 J4]].
+  exists (SBnsop.mkState S' TD' Ps' 
+    ((SBnsop.mkEC f1' (block_intro l' ps' cs' tmn') cs' tmn' lc2' rm' als1')
+      ::ECs') gl' fs' M' MM').
+  split; eauto.
+    repeat (split; auto).
+Case "dsBranch_uncond". simpl_nd_sbds. 
+  eapply instantiate_locals__switchToNewBasicBlock in H0; eauto.
+  destruct H0 as [lc2' [J1 J2]]. 
+  exists (SBnsop.mkState S' TD' Ps' 
+    ((SBnsop.mkEC f1' (block_intro l' ps' cs' tmn') cs' tmn' lc2' rm' als1')
+      ::ECs') gl' fs' M' MM').
+  split; eauto.
+    repeat (split; auto).
+Case "dsBop". simpl_nd_sbds. 
+  eapply instantiate_locals__BOP in H; eauto.
+  destruct H as [gvs3' [J1 J2]].
+  exists (SBnsop.mkState S' TD' Ps' 
+    ((SBnsop.mkEC f1' b1' cs tmn1' (updateAddAL _ lc1' id0 gvs3') rm1' als1')
+      ::ECs') gl' fs' M' MM').
+  split; eauto.
+    repeat (split; auto using instantiate_locals__updateAddAL).
+Case "dsFBop". simpl_nd_sbds. 
+  eapply instantiate_locals__FBOP in H; eauto.
+  destruct H as [gvs3' [J1 J2]]. 
+  exists (SBnsop.mkState S' TD' Ps' 
+    ((SBnsop.mkEC f1' b1' cs tmn1' (updateAddAL _ lc1' id0 gvs3') rm1' als1')
+      ::ECs') gl' fs' M' MM').
+  split; eauto.
+    repeat (split; auto using instantiate_locals__updateAddAL).
+Case "dsExtractValue". simpl_nd_sbds. 
+  eapply instantiate_locals__getOperandValue in H; eauto.
+  destruct H as [gvs [J1 J2]].
+  eapply instantiate_locals__extractGenericValue in H0; eauto.
+  destruct H0 as [gvs' [J3 J4]].
+  exists (SBnsop.mkState S' TD' Ps' 
+    ((SBnsop.mkEC f1' b1' cs tmn1' (updateAddAL _ lc1' id0 gvs') rm1' als1')
+      ::ECs') gl' fs' M' MM').
+  split; eauto.
+    repeat (split; auto using instantiate_locals__updateAddAL).
+Case "dsInsertValue". simpl_nd_sbds. 
+  eapply instantiate_locals__getOperandValue in H; eauto.
+  destruct H as [gvs [J1 J2]].
+  eapply instantiate_locals__getOperandValue in H0; eauto.
+  destruct H0 as [gvs' [J1' J2']].
+  eapply instantiate_locals__insertGenericValue in H1; eauto.
+  destruct H1 as [gvs'' [J3 J4]].
+  exists (SBnsop.mkState S' TD' Ps' 
+    ((SBnsop.mkEC f1' b1' cs tmn1' (updateAddAL _ lc1' id0 gvs'') rm1' als1')
+      ::ECs') gl' fs' M' MM').
+  split; eauto.
+    repeat (split; auto using instantiate_locals__updateAddAL).
+Case "dsMalloc". simpl_nd_sbds. 
+  eapply instantiate_locals__getOperandValue in H0; eauto.
+  destruct H0 as [gns [J1 J2]].
+  exists (SBnsop.mkState S' TD' Ps' 
+    ((SBnsop.mkEC f1' b1' cs tmn1' 
+      (updateAddAL _ lc1' id0 ($ (blk2GV TD' mb) # typ_pointer t $)) 
+    rm' als1')::ECs') gl' fs' Mem' MM').
+  inv H3.
+  split; eauto.
+    repeat (split; auto using instantiate_locals__updateAddAL, 
+                              instantiate_gv__gv2gvs).
+Case "dsFree". simpl_nd_sbds. 
+  eapply instantiate_locals__getOperandValue in H; eauto.
+  destruct H as [gvs [J1 J2]].
+  exists (SBnsop.mkState S' TD' Ps' 
+    ((SBnsop.mkEC f1' b1' cs tmn1' lc1' rm1'
+    als1')::ECs') gl' fs' Mem' MM').
+  split; eauto. 
+    repeat (split; auto).
+Case "dsAlloca". simpl_nd_sbds. 
+  eapply instantiate_locals__getOperandValue in H0; eauto.
+  destruct H0 as [gns [J1 J2]].
+  exists (SBnsop.mkState S' TD' Ps' 
+    ((SBnsop.mkEC f1' b1' cs tmn1' 
+      (updateAddAL _ lc1' id0 ($ (blk2GV TD' mb) # typ_pointer t $)) rm'
+    (mb::als1'))::ECs') gl' fs' Mem' MM').
+  inv H3.
+  split; eauto.
+    repeat (split; auto using instantiate_locals__updateAddAL, 
+                              instantiate_gv__gv2gvs).
+Case "dsLoad_nptr". simpl_nd_sbds.
+  eapply instantiate_locals__getOperandValue in H0; eauto.
+  destruct H0 as [gvs2 [J1 J2]].
+  exists (SBnsop.mkState S' TD' Ps' 
+    ((SBnsop.mkEC f1' b1' cs tmn1' (updateAddAL _ lc1' id0 ($ gv # t $))
+    rm1' als1')::ECs') gl' fs' M' MM').
+  split; eauto. 
+    repeat (split; auto using instantiate_locals__updateAddAL, 
+                              instantiate_gv__gv2gvs).
+Case "dsLoad_ptr". simpl_nd_sbds.
+  eapply instantiate_locals__getOperandValue in H0; eauto.
+  destruct H0 as [gvs2 [J1 J2]].
+  exists (SBnsop.mkState S' TD' Ps' 
+    ((SBnsop.mkEC f1' b1' cs tmn1' (updateAddAL _ lc1' id0 ($ gv # t $))
+    rm' als1')::ECs') gl' fs' M' MM').
+  inv H5.
+  split; eauto. 
+    repeat (split; auto using instantiate_locals__updateAddAL, 
+                              instantiate_gv__gv2gvs).
+Case "dsStore_nptr". simpl_nd_sbds.
+  eapply instantiate_locals__getOperandValue in H0; eauto.
+  destruct H0 as [gvs2 [J1 J2]].
+  eapply instantiate_locals__getOperandValue in H1; eauto.
+  destruct H1 as [mps2 [J3 J4]].
+  exists (SBnsop.mkState S' TD' Ps' 
+    ((SBnsop.mkEC f1' b1' cs tmn1' lc1' rm1' als1')::ECs') gl' fs' Mem' MM').
+  split; eauto. 
+    repeat (split; auto).
+Case "dsStore_ptr". 
+  rename MM' into MM0. simpl_nd_sbds.
+  eapply instantiate_locals__getOperandValue in H0; eauto.
+  destruct H0 as [gvs2 [J1 J2]].
+  eapply instantiate_locals__getOperandValue in H1; eauto.
+  destruct H1 as [mps2 [J3 J4]].
+  exists (SBnsop.mkState S' TD' Ps' 
+    ((SBnsop.mkEC f1' b1' cs tmn1' lc1' rm1' als1')::ECs') gl' fs' Mem' 
+      (set_mem_metadata TD' MM' gvp md')).
+  split; eauto. 
+    repeat (split; auto).
+Case "dsGEP". simpl_nd_sbds. 
+  eapply instantiate_locals__getOperandValue in H0; eauto.
+  destruct H0 as [mps [J1 J2]].
+  eapply instantiate_locals__values2GVs in H1; eauto.
+  destruct H1 as [vidxss [J3 J4]].
+  eapply instantiate_locals__GEP in H2; eauto.
+  destruct H2 as [mps2' [J5 J6]].
+  exists (SBnsop.mkState S' TD' Ps' 
+    ((SBnsop.mkEC f1' b1' cs tmn1' (updateAddAL _ lc1' id0 mps2') rm' als1')
+      ::ECs') gl' fs' M' MM').
+  inv H3.
+  split; eauto.
+    repeat (split; auto using instantiate_locals__updateAddAL).
+Case "dsTrunc". simpl_nd_sbds.
+  eapply instantiate_locals__TRUNC in H; eauto.
+  destruct H as [gvs2' [J1 J2]].
+  exists (SBnsop.mkState S' TD' Ps' 
+    ((SBnsop.mkEC f1' b1' cs tmn1' (updateAddAL _ lc1' id0 gvs2') rm1' als1')
+      ::ECs') gl' fs' M' MM').
+  split; eauto.
+    repeat (split; auto using instantiate_locals__updateAddAL).
+Case "dsExt". simpl_nd_sbds. 
+  eapply instantiate_locals__EXT in H; eauto.
+  destruct H as [gvs2' [J1 J2]].
+  exists (SBnsop.mkState S' TD' Ps' 
+    ((SBnsop.mkEC f1' b1' cs tmn1' (updateAddAL _ lc1' id0 gvs2') rm1' als1')
+      ::ECs') gl' fs' M' MM').
+  split; eauto.
+    repeat (split; auto using instantiate_locals__updateAddAL).
+Case "dsBitcast_nptr". simpl_nd_sbds. 
+  eapply instantiate_locals__CAST in H; eauto.
+  destruct H as [gvs2' [J1 J2]].
+  exists (SBnsop.mkState S' TD' Ps' 
+    ((SBnsop.mkEC f1' b1' cs tmn1' (updateAddAL _ lc1' id0 gvs2') rm1' als1')
+      ::ECs') gl' fs' M' MM').
+  split; eauto.
+    repeat (split; auto using instantiate_locals__updateAddAL).
+Case "dsBitcast_ptr". simpl_nd_sbds. 
+  eapply instantiate_locals__CAST in H; eauto.
+  destruct H as [gvs2' [J1 J2]].
+  exists (SBnsop.mkState S' TD' Ps' 
+    ((SBnsop.mkEC f1' b1' cs tmn1' (updateAddAL _ lc1' id0 gvs2') rm' als1')
+      ::ECs') gl' fs' M' MM').
+  inv H2.
+  split; eauto.
+    repeat (split; auto using instantiate_locals__updateAddAL).
+Case "dsInttoptr". simpl_nd_sbds. 
+  eapply instantiate_locals__CAST in H; eauto.
+  destruct H as [gvs2' [J1 J2]].
+  exists (SBnsop.mkState S' TD' Ps' 
+    ((SBnsop.mkEC f1' b1' cs tmn1' (updateAddAL _ lc1' id0 gvs2') rm' als1')
+      ::ECs') gl' fs' M' MM').
+  inv H0.
+  split; eauto.
+    repeat (split; auto using instantiate_locals__updateAddAL).
+Case "dsOthercast". simpl_nd_sbds. 
+  eapply instantiate_locals__CAST in H; eauto.
+  destruct H as [gvs2' [J1 J2]].
+  exists (SBnsop.mkState S' TD' Ps' 
+    ((SBnsop.mkEC f1' b1' cs tmn1' (updateAddAL _ lc1' id0 gvs2') rm1' als1')
+      ::ECs') gl' fs' M' MM').
+  split; eauto.
+    repeat (split; auto using instantiate_locals__updateAddAL).
+Case "dsIcmp". simpl_nd_sbds. 
+  eapply instantiate_locals__ICMP in H; eauto.
+  destruct H as [gvs3' [J1 J2]].
+  exists (SBnsop.mkState S' TD' Ps' 
+    ((SBnsop.mkEC f1' b1' cs tmn1' (updateAddAL _ lc1' id0 gvs3') rm1' als1')
+      ::ECs') gl' fs' M' MM').
+  split; eauto.
+    repeat (split; auto using instantiate_locals__updateAddAL).
+Case "dsFcmp". simpl_nd_sbds. 
+  eapply instantiate_locals__FCMP in H; eauto.
+  destruct H as [gvs3' [J1 J2]]. 
+  exists (SBnsop.mkState S' TD' Ps' 
+    ((SBnsop.mkEC f1' b1' cs tmn1' (updateAddAL _ lc1' id0 gvs3') rm1' als1')
+      ::ECs') gl' fs' M' MM').
+  split; eauto.
+    repeat (split; auto using instantiate_locals__updateAddAL).
+Case "dsSelect_nptr". simpl_nd_sbds. 
+  eapply instantiate_locals__getOperandValue in H; eauto.
+  destruct H as [gvs0' [J1 J2]].
+  eapply instantiate_locals__getOperandValue in H0; eauto.
+  destruct H0 as [gvs1' [J3 J4]].
+  eapply instantiate_locals__getOperandValue in H1; eauto.
+  destruct H1 as [gvs2' [J5 J6]].
+  exists (SBnsop.mkState S' TD' Ps' 
+    ((SBnsop.mkEC f1' b1' cs tmn1' (if isGVZero TD' c 
+                                   then updateAddAL _ lc1' id0 gvs2' 
+                                   else updateAddAL _ lc1' id0 gvs1') rm1' als1')
+      ::ECs') gl' fs' M' MM').
+  split; eauto.
+    repeat (split; auto).
+      destruct (isGVZero TD' c); auto using instantiate_locals__updateAddAL.
+Case "dsSelect_ptr". simpl_nd_sbds. 
+  eapply instantiate_locals__getOperandValue in H; eauto.
+  destruct H as [gvs0' [J1 J2]].
+  eapply instantiate_locals__getOperandValue in H0; eauto.
+  destruct H0 as [gvs1' [J3 J4]].
+  eapply instantiate_locals__getOperandValue in H1; eauto.
+  destruct H1 as [gvs2' [J5 J6]].
+  exists (SBnsop.mkState S' TD' Ps' 
+    ((SBnsop.mkEC f1' b1' cs tmn1' (if isGVZero TD' c 
+                                   then updateAddAL _ lc1' id0 gvs2' 
+                                   else updateAddAL _ lc1' id0 gvs1') rm' als1')
+      ::ECs') gl' fs' M' MM').
+  split.
+    eapply SBnsop.nsSelect_ptr; eauto.
+      destruct (isGVZero TD' c); inv H5; eauto.
+  repeat (split; auto).
+    destruct (isGVZero TD' c); inv H5; 
+      auto using instantiate_locals__updateAddAL.
+Case "dsCall". simpl_nd_sbds. 
+  apply lookupFdefViaGV_inversion in H.
+  destruct H as [fptr [fn [J1 [J2 J3]]]].
+  eapply instantiate_locals__getOperandValue in J1; eauto.
+  destruct J1 as [gvs2 [J11 J12]].
+  eapply instantiate_locals__params2GVs in H1; eauto.
+  destruct H1 as [gvss2 [H11 H12]].
+  eapply instantiate_locals__initLocals in H2; eauto.
+  destruct H2 as [lc2' [H21 H22]].
+  exists (SBnsop.mkState S' TD' Ps' 
+    ((SBnsop.mkEC (fdef_intro (fheader_intro fa rt fid la va) lb) 
+                       (block_intro l' ps' cs' tmn') cs' tmn' 
+                       lc2' rm'
+                       nil)::
+     (SBnsop.mkEC f1' b1' (insn_call rid noret0 ca ft fv lp :: cs) tmn1' 
+      lc1' rm1' als1') ::ECs') gl' fs' M' MM').
+  split.
+    eapply SBnsop.nsCall; eauto.
+      unfold lookupFdefViaPtr. 
+      rewrite J2. simpl. rewrite J3. auto.
+    repeat (split; auto).
+Case "dsExCall". simpl_nd_sbds. 
+  apply lookupExFdecViaGV_inversion in H.
+  destruct H as [fptr [fn [J1 [J2 [J3 J4]]]]].
+  eapply instantiate_locals__getOperandValue in J1; eauto.
+  destruct J1 as [gvs2 [J11 J12]].
+  eapply ndopsem_dsop.instantiate_locals__params2GVs in H0; eauto.
+  destruct H0 as [gvss2 [H11 H12]].
+  eapply instantiate_locals__exCallUpdateLocals in H2; eauto.
+  destruct H2 as [lc2' [H21 H22]].
+  exists (SBnsop.mkState S' TD' Ps' 
+    ((SBnsop.mkEC f1' b1' cs tmn1' lc2' rm' als1') ::ECs') gl' fs' Mem' MM').
+  split.
+    eapply SBnsop.nsExCall; eauto.
+      unfold lookupExFdecViaPtr. 
+      rewrite J2. simpl. rewrite J3. rewrite J4. eauto.
+    repeat (split; auto).
+Qed.
+
+
+(*****************************)
+(*
+*** Local Variables: ***
+*** coq-prog-name: "coqtop" ***
+*** coq-prog-args: ("-emacs-U" "-I" "~/SVN/sol/vol/src/ssa/monads" "-I" "~/SVN/sol/vol/src/ssa/ott" "-I" "~/SVN/sol/vol/src/ssa/compcert" "-I" "~/SVN/sol/theory/metatheory_8.3" "-I" "~/SVN/sol/vol/src/TV") ***
+*** End: ***
+ *)
+
