src/SoftBound/sb_ns_metadata.v
@@ -29,6 +29,8 @@ Require Import ssa_analysis.
 Require Import ssa_wf.
 Require Import ssa_dynamic.
 Require Import ndopsem.
+Require Import sb_ds_def.
+Require Import sb_ds_metadata.
 Require Import sb_ns_def.
 Require Import sbop_nsop.
 Require Import Znumtheory.
@@ -70,23 +72,7 @@ Export SBnsop.
 
 (*****************************************)
 (* misc *)
-Lemma GV2ptr_base2GV : forall TD mb,
-  GV2ptr TD (getPointerSize TD) (base2GV TD mb) = 
-    Some (Values.Vptr mb (Int.repr 31 0)).
-Proof.
-  intros TD mb.
-  unfold GV2ptr. unfold base2GV. unfold blk2GV. unfold ptr2GV. unfold val2GV.
-  auto.
-Qed.
 
-Lemma GV2ptr_bound2GV : forall TD mb tsz n,
-  GV2ptr TD (getPointerSize TD) (bound2GV TD mb tsz n) = 
-    Some (Values.Vptr mb (Int.repr 31 ((Size.to_Z tsz)*n))).
-Proof.
-  intros TD mb tsz n.
-  unfold GV2ptr. unfold bound2GV. unfold ptr2GV. unfold val2GV.
-  auto.
-Qed.
 Lemma updateValuesForNewBlock_spec4 : forall rvs lc x rm lc' rm' md,
   lookupAL _ rm x = None ->
   (lc', rm') = updateValuesForNewBlock rvs lc rm ->
@@ -157,7 +143,7 @@ Proof.
     destruct R; try solve [inv H].
     simpl.
     destruct (isPointerTypB t); inv H.
-      destruct (get_reg_metadata TD gl rm v) as [[md mt]|]; inv H2.      
+      destruct (SBopsem.get_reg_metadata TD gl rm v) as [[md mt]|]; inv H2.      
       simpl in H0.
       destruct H0 as [H0 | H0]; eauto.  
         inv H0; auto.
@@ -265,7 +251,7 @@ Lemma initializeFrameValues_spec3 : forall la lc x rm lc' rm' md,
   (lc', rm') = _initializeFrameValues la nil lc rm ->
   lookupAL _ rm' x = Some md ->
   lookupAL _ rm x = Some md \/
-  md = mkMD null null.
+  md = SBopsem.mkMD null null.
 Proof.
   induction la; simpl; intros.
     inv H. auto.
@@ -287,7 +273,7 @@ Lemma initializeFrameValues_spec2 : forall la ogvs lc x rm lc' rm' md,
   (lc', rm') = _initializeFrameValues la ogvs lc rm ->
   lookupAL _ rm' x = Some md ->
   lookupAL _ rm x = Some md \/
-  md = mkMD null null \/
+  md = SBopsem.mkMD null null \/
   exists gv1, In (gv1,Some md) ogvs.
 Proof.
   induction la; simpl; intros ogvs lc x rm lc' rm' md Hinit Hlk.
@@ -336,260 +322,8 @@ Proof.
           right. right. exists gv1. simpl. auto.
 Qed.
 
-(*****************************************)
-(* wf_data *)
-
-Definition blk_temporal_safe M b : Prop :=
-let (lo, _) := Mem.bounds M b in
-Mem.perm M b lo Nonempty.
-
-Definition wf_data (TD:TargetData) (M:mem) (gvb gve:GenericValue) : Prop :=
-  match (GV2ptr TD (getPointerSize TD) gvb,
-         GV2ptr TD (getPointerSize TD) gve) with
-  | (Some (Values.Vptr bb bofs), Some (Values.Vptr eb eofs)) =>
-      if zeq bb eb then
-        bb < Mem.nextblock M /\
-        (blk_temporal_safe M bb ->
-         Mem.range_perm M bb (Int.signed 31 bofs) (Int.signed 31 eofs) Writable)
-      else False
-  | _ => False
-  end.
-
-Definition wf_rmetadata (TD:TargetData) (M:mem) (rm:rmetadata) : Prop :=
-  forall (i:id) (gvb gve:GenericValue),
-    lookupAL _ rm i = Some (mkMD gvb gve) -> wf_data TD M gvb gve.
-
-Definition wf_mmetadata (TD:TargetData) (M:mem) (MM:mmetadata) : Prop :=
-  forall (b:Values.block) (ofs:int32) (gvb gve:GenericValue),
-    MM b ofs = Some (mkMD gvb gve) -> wf_data TD M gvb gve.
-
-Definition wf_metadata (TD:TargetData) (M:mem) (rm:rmetadata) (MM:mmetadata) 
-    : Prop :=
-  wf_rmetadata TD M rm /\ wf_mmetadata TD M MM.
-
-Definition wf_global_ptr S TD Mem0 gl : Prop :=
-  forall id0 gv0 typ0, lookupAL GenericValue gl id0 = Some gv0 ->
-  wf_const S TD (const_gid typ0 id0) (typ_pointer typ0) ->
-  exists b, exists sz,
-    GV2ptr TD (getPointerSize TD) gv0 = Some (Values.Vptr b ((Int.zero 31))) /\
-    getTypeAllocSize TD typ0 = Some sz /\
-    Mem.bounds Mem0 b = (0, Z_of_nat sz) /\
-    b < Mem.nextblock Mem0 /\
-    (blk_temporal_safe Mem0 b -> Mem.range_perm Mem0 b 0 (Z_of_nat sz) Writable).
-
-(***********************************************)
-(* axiom *)
-
-Axiom callExternalFunction_mem_bounds : forall Mem0 fid gvs oresult Mem' b,
-  callExternalFunction Mem0 fid gvs = Some (oresult, Mem') ->
-  Mem.bounds Mem0 b = Mem.bounds Mem' b.
-
-Axiom callExternalFunction_temporal_prop : forall Mem0 fid gvs oresult Mem' base
-    bound b,
-  callExternalFunction Mem0 fid gvs = Some (oresult, Mem') ->
-  b < Mem.nextblock Mem0 /\
-  (blk_temporal_safe Mem0 b -> Mem.range_perm Mem0 b base bound Writable) ->
-  b < Mem.nextblock Mem' /\
-  (blk_temporal_safe Mem' b -> Mem.range_perm Mem' b base bound Writable).
-
-(***********************************************)
-(* dec *)
-
-Lemma assert_mptr_dec : forall TD t ptr md,
-  assert_mptr TD t ptr md \/ ~ assert_mptr TD t ptr md.
-Proof.
-  intros.
-  unfold is_true. 
-  destruct (assert_mptr TD t ptr md); auto.
-Qed.
-
-Lemma blk_temporal_safe_dec : forall M b,
-  {blk_temporal_safe M b} + {~ blk_temporal_safe M b}.
-Proof.
-  intros M b.
-  unfold blk_temporal_safe.
-  destruct (Mem.bounds M b).
-  apply Mem.perm_dec.
-Qed.
-
-Lemma valid_block_dec : forall M b,
-  {Mem.valid_block M b} + { ~ Mem.valid_block M b}.
-Proof.
-  intros M b.
-  unfold Mem.valid_block.
-  apply Z_lt_dec; auto.
-Qed.  
-
-(***********************************************)
-(* temoporal_prop *)
-
-Lemma blk_temporal_safe_store_2 : forall m Mem0 b ofs0 v0 Mem' b0,
-  Mem.store m Mem0 b ofs0 v0 = Some Mem' ->
-  blk_temporal_safe Mem' b0 ->
-  blk_temporal_safe Mem0 b0. 
-Proof.
-  intros m Mem0 b ofs0 v0 Mem' b0 Hstore H.
-  unfold blk_temporal_safe in *.
-  assert (J:=Hstore).
-  apply Mem.bounds_store with (b':=b0) in J.
-  rewrite <- J.
-  destruct (Mem.bounds Mem' b0).
-  eapply Mem.perm_store_2 in H; eauto.  
-Qed.
-
-Lemma store_preserves_temoporal_prop : forall m Mem0 b b1 ofs0 v0 Mem' i0 i1
-  (H1 : Mem.store m Mem0 b ofs0 v0 = Some Mem')
-  (J : b1 < Mem.nextblock Mem0 /\
-      (blk_temporal_safe Mem0 b1 ->
-       Mem.range_perm Mem0 b1 i0 i1 Writable)),
-  b1 < Mem.nextblock Mem' /\
-   (blk_temporal_safe Mem' b1 ->
-    Mem.range_perm Mem' b1 i0 i1 Writable).
-Proof.
-  intros.
-    destruct J as [J1 J2].
-    split.
-      apply Mem.nextblock_store in H1.
-      rewrite H1. auto.
-
-      intro H.
-      eapply blk_temporal_safe_store_2 in H; eauto.
-      apply J2 in H.
-      eauto using Mem.store_range_perm_1.
-Qed.
-
-Lemma free_preserves_temporal_prop : forall (Mem0 Mem' : mem) (b : Values.block)
-  (z z0 : Z) (HeqR : (z, z0) = Mem.bounds Mem0 b)
-  (H0 : Mem.free Mem0 b z z0 = ret Mem')
-  (i0 : Z) (b1 : Values.block) (i1 : Z)
-  (J2 : b1 < Mem.nextblock Mem0 /\ 
-        (blk_temporal_safe Mem0 b1 -> Mem.range_perm Mem0 b1 i0 i1 Writable)),
-  b1 < Mem.nextblock Mem' /\
-  (blk_temporal_safe Mem' b1 -> Mem.range_perm Mem' b1 i0 i1 Writable).
-Proof.
-  intros. 
-  destruct J2 as [J2 J3].
-  split.
-      apply Mem.nextblock_free in H0.
-      rewrite H0. auto.
-
-      intro Hwfb.
-      unfold blk_temporal_safe in *.
-      erewrite Mem.bounds_free in Hwfb; eauto.
-      assert (Hfree:=H0).
-      destruct (Values.eq_block b b1); subst.
-        rewrite <- HeqR in Hwfb.
-        destruct (Z_lt_dec z z0).
-          apply Mem.perm_free_2 with (ofs:=z)(p:=Nonempty) in H0; 
-            zeauto.
-          contradict Hwfb; auto.
-
-          rewrite <- HeqR in J3.   
-          eapply Mem.perm_free_3 in Hwfb; eauto.
-          apply J3 in Hwfb. clear J3.
-          unfold Mem.range_perm in *.
-          intros ofs J. apply Hwfb in J.
-          apply Mem.perm_free_1 with (b:=b1)(ofs:=ofs)(p:=Writable) in H0; auto.
-            clear - n.
-            destruct (Z_lt_dec ofs z); auto.
-            destruct (Z_le_dec z0 ofs); auto.
-            assert (False) as H. zeauto. 
-            inversion H.
-
-       destruct (Mem.bounds Mem0 b1).
-       eapply Mem.perm_free_3 in Hwfb; eauto.
-       apply J3 in Hwfb. clear J3.
-       unfold Mem.range_perm in *.
-       intros ofs J. apply Hwfb in J.
-        apply Mem.perm_free_1 with (b:=b1)(ofs:=ofs)(p:=Writable) in H0;
-          zeauto.
-Qed.     
-
-Lemma blk_temporal_alloc_inv : forall Mem0 lo hi Mem' mb b0,
-  Mem.alloc Mem0 lo hi = (Mem', mb) ->
-  blk_temporal_safe Mem' b0 ->
-  (if Values.eq_block b0 mb then 
-    Mem.bounds Mem' b0 = (lo, hi)
-  else blk_temporal_safe Mem0 b0).
-Proof.
-  intros.
-  unfold blk_temporal_safe in *.
-  assert (Halloc := H).  
-  apply Mem.bounds_alloc with (b':=b0) in H.
-  destruct (Values.eq_block b0 mb); subst; auto.
-    rewrite <- H.
-    destruct (Mem.bounds Mem' b0).
-    apply Mem.perm_alloc_inv with (b':=b0)(ofs:=z)(p:=Nonempty) in Halloc; auto.
-    destruct (zeq b0 mb); auto.
-      subst. contradict n; auto.
-Qed.
-
-Lemma alloc_preserves_temporal_prop : forall Mem0 sz Mem' mb
-  (H4 : Mem.alloc Mem0 0 sz = (Mem', mb))
-  (i0 : Z) (b0 : Values.block) (i1 : Z)
-  (J' : b0 < Mem.nextblock Mem0 /\ 
-        (blk_temporal_safe Mem0 b0 -> Mem.range_perm Mem0 b0 i0 i1 Writable)),
-  b0 < Mem.nextblock Mem' /\
-  (blk_temporal_safe Mem' b0 -> Mem.range_perm Mem' b0 i0 i1 Writable).
-Proof.
-  intros.
-  destruct J' as [J1' J2'].
-  split.
-    apply Mem.nextblock_alloc in H4.
-    rewrite H4. zauto.
-
-    intro Hwfb.
-    assert (Halloc := H4).
-    eapply blk_temporal_alloc_inv in H4; eauto.         
-    destruct (Values.eq_block b0 mb); subst.
-      apply Mem.alloc_result in Halloc.    
-      rewrite <- Halloc in J1'.
-      contradict J1'; zauto.
-      
-      apply J2' in H4.
-      eauto using Mem.range_perm_alloc_other.
-Qed.
-
 (***********************************************)
 (* wf_data *)
-
-Lemma wf_mmetadata__wf_data : forall Mem0 TD MM b0 ofs gvb gve,
-  wf_mmetadata TD Mem0 MM ->
-  MM b0 ofs = Some (mkMD gvb gve) ->
-  wf_data TD Mem0 gvb gve.
-Proof.
-  intros Mem0 TD MM b0 ofs gvb gve Hwfm J.
-  apply Hwfm in J; clear Hwfm.
-  unfold wf_data in *.
-  destruct (GV2ptr TD (getPointerSize TD) gvb); auto.
-Qed.
-
-Lemma wf_data__store__wf_data : forall m Mem0 b ofs0 v0 Mem' TD gvb gve,
-  Mem.store m Mem0 b ofs0 v0 = Some Mem' ->
-  wf_data TD Mem0 gvb gve ->
-  wf_data TD Mem' gvb gve.
-Proof.
-  intros m Mem0 b ofs0 v0 Mem' TD gvb gve H1 J.
-  unfold wf_data in *.
-  destruct (GV2ptr TD (getPointerSize TD) gvb); auto.
-  destruct v; auto.
-  destruct (GV2ptr TD (getPointerSize TD) gve); auto.
-  destruct v; auto.
-  destruct (zeq b0 b1); subst; auto.
-    eapply store_preserves_temoporal_prop; eauto.
-Qed.
-
-Lemma wf_mmetadata__store__wf_data : forall m Mem0 b ofs0 v0 Mem' TD MM b0 ofs 
-    gvb gve,
-  Mem.store m Mem0 b ofs0 v0 = Some Mem' ->
-  wf_mmetadata TD Mem0 MM ->
-  MM b0 ofs = Some (mkMD gvb gve) ->
-  wf_data TD Mem' gvb gve.
-Proof.
-  intros m Mem0 b ofs0 v0 Mem' TD MM b0 ofs gvb gve H1 Hwfm J.
-  apply wf_mmetadata__wf_data with (Mem0:=Mem0)(TD:=TD) in J; eauto.
-  eapply wf_data__store__wf_data; eauto.
-Qed.
 
 Lemma GV2ptr__cgv2gv : forall TD sz g b ofs t, 
   GV2ptr TD sz g = ret (Vptr b ofs) -> g = ? g # typ_pointer t ?.
@@ -693,26 +427,6 @@ Proof.
     contradict J; zauto.
 Qed.
 
-Lemma nullptr_lt_nextblock : forall Mem0,
-  Mem.nullptr < Mem.nextblock Mem0.
-Proof.
-  intros.
-  assert (J:=@Mem.nextblock_pos Mem0).
-  unfold Mem.nullptr.
-  zauto.
-Qed.
-
-Lemma null_is_wf_data : forall TD Mem,
-  wf_data TD Mem null null.
-Proof.
-  intros TD Mem.
-  eapply eq_gv_is_wf_data with (bb:=Mem.nullptr).
-    apply nullptr_lt_nextblock.
-
-    unfold GV2ptr.
-    simpl. eauto.
-Qed.
-
 Lemma wf_rmetadata__get_const_metadata : forall S TD gl Mem0 rm c gvb gve c0 c1
    ct',
   wf_global_ptr S TD Mem0 gl ->
@@ -764,310 +478,8 @@ Proof.
   simpl in H1; eauto.
 Qed.
 
-Lemma wf_rmetadata__get_reg_metadata : forall S los nts Ps Mem0 rm gl vp gvb gve 
-    f tp,
-  wf_global_ptr S (los, nts) Mem0 gl ->
-  wf_rmetadata (los, nts) Mem0 rm ->
-  wf_value S (module_intro los nts Ps) f vp tp ->
-  get_reg_metadata (los, nts) gl rm vp = Some (mkMD gvb gve) ->
-  wf_data (los, nts) Mem0 gvb gve.
-Proof.
-  intros S los nts Ps Mem0 rm gl vp gvb gve t tp Hwfg Hwfr Hwfv J.
-  unfold get_reg_metadata in J.
-  destruct vp.
-    remember (lookupAL metadata rm i0) as R.
-    destruct R; inv J.
-    symmetry in HeqR.
-    apply Hwfr in HeqR; auto.
-
-    remember (get_const_metadata c) as R.
-    destruct R as [[bc ec] |]; 
-      try solve [inversion J; subst; auto using null_is_wf_data].
-    remember (const2GV (los, nts) gl bc) as R0.
-    remember (const2GV (los, nts) gl ec) as R1.
-    destruct R0; try solve [inversion J]. 
-    simpl in J.
-    destruct R1; try solve [inversion J]. 
-    simpl in J.
-    inv J.
-    inv Hwfv.
-    eapply wf_rmetadata__get_const_metadata; eauto.
-Qed.
-
-Lemma wf_mmetadata__get_mem_metadata : forall TD Mem0 MM gvp gvb gve,
-  wf_mmetadata TD Mem0 MM ->
-  get_mem_metadata TD MM gvp = mkMD gvb gve ->
-  wf_data TD Mem0 gvb gve.
-Proof.
-  intros TD Mem0 MM gvp gvb gve Hwfm H4.
-  unfold get_mem_metadata in H4.
-  remember (GV2ptr TD (getPointerSize TD) gvp) as R.
-  destruct R; try solve [inversion H4; subst; auto using null_is_wf_data].
-  destruct v; try solve [inversion H4; subst; auto using null_is_wf_data].
-  remember (MM b i0) as R'.
-  destruct R'; inv H4; auto using null_is_wf_data.
-  symmetry in HeqR'.     
-  apply Hwfm in HeqR'; auto.
-Qed.
-
-Lemma free_preserves_wf_data : forall TD (Mem0 Mem' : mem) (b : Values.block)
-  (z z0 : Z) (HeqR : (z, z0) = Mem.bounds Mem0 b)
-  (H0 : Mem.free Mem0 b z z0 = ret Mem') (gvb gve : GenericValue)
-  (J : wf_data TD Mem0 gvb gve),
-  wf_data TD Mem' gvb gve.
-Proof.
-  intros.
-    unfold wf_data in *.
-    remember (GV2ptr TD (getPointerSize TD) gvb) as Rb.
-    destruct Rb; auto.
-    destruct v; auto.
-    remember (GV2ptr TD (getPointerSize TD) gve) as Re.
-    destruct Re; auto.
-    destruct v; auto.
-    destruct (zeq b0 b1); subst; auto. 
-    destruct J as [J1 J2].
-    split.
-      apply Mem.nextblock_free in H0.
-      rewrite H0. auto.
-
-      eapply free_preserves_temporal_prop; eauto.
-Qed.
-
-Lemma alloc_preserves_wf_data : forall TD Mem0 sz Mem' mb
-  (H4 : Mem.alloc Mem0 0 sz = (Mem', mb))
-  (gvb : GenericValue)
-  (gve : GenericValue)
-  (J' : wf_data TD Mem0 gvb gve),
-  wf_data TD Mem' gvb gve.
-Proof.
-  intros.
-  unfold wf_data in *.
-  remember (GV2ptr TD (getPointerSize TD) gvb) as Rb.
-  destruct Rb; auto.
-  destruct v; auto.
-  remember (GV2ptr TD (getPointerSize TD) gve) as Re.
-  destruct Re; auto.
-  destruct v; auto.
-  destruct (zeq b b0); subst; auto. 
-    eapply alloc_preserves_temporal_prop; eauto.
-Qed.
-
-(****************************************)
-(* wf_global_ptr *)
-
-Lemma free_preserves_wf_global_ptr : forall S TD Mem0 gl gv Mem',
-  free TD Mem0 gv = ret Mem' ->
-  wf_global_ptr S TD Mem0 gl ->
-  wf_global_ptr S TD Mem' gl.
-Proof.
-  intros S TD Mem0 gl gv Mem' Hfree Hwfg.
-  apply free_inv in Hfree. 
-  destruct Hfree as [blk [ofs [hi [lo [J1 [J2 [J3 J4]]]]]]].
-  intros x gv0 typ0 Hlk Hwfc.
-  eapply Hwfg in Hwfc; eauto.
-  destruct Hwfc as [b [sz0 [J5 [J6 [J7 J8]]]]].
-  eapply free_preserves_temporal_prop in J8; eauto.
-  exists b. exists sz0. repeat (split; auto).
-    erewrite Mem.bounds_free; eauto.
-Qed.
-
-Lemma free_allocas_preserves_wf_global_ptr : forall S TD gl als Mem0 Mem',
-  free_allocas TD Mem0 als = ret Mem' ->
-  wf_global_ptr S TD Mem0 gl ->
-  wf_global_ptr S TD Mem' gl.
-Proof.  
-  induction als; simpl; intros Mem0 Mem' Hfree Hwfr.
-    inv Hfree. auto.
-
-    remember (free TD Mem0 (blk2GV TD a)) as R.
-    destruct R; inv Hfree.
-    eapply IHals; eauto.
-    eapply free_preserves_wf_global_ptr in Hwfr; eauto.
-Qed.
-
-Lemma malloc_preserves_wf_global_ptr : forall S TD Mem0 gl tsz gn align0 Mem' mb,
-  malloc TD Mem0 tsz gn align0 = ret (Mem', mb) ->
-  wf_global_ptr S TD Mem0 gl ->
-  wf_global_ptr S TD Mem' gl.
-Proof.
-  intros.
-  apply malloc_inv in H.
-  destruct H as [n [J1 [J0 J2]]].
-  intros x gv0 typ0 Hlk Hwfc.
-  eapply H0 in Hwfc; eauto.
-  destruct Hwfc as [b [sz0 [J5 [J6 [J3 J4]]]]].
-  exists b. exists sz0.
-  assert (G:=J4). destruct G as [G _].
-  eapply alloc_preserves_temporal_prop in J4; eauto.
-  repeat (split; auto).
-    assert (J:=J2).
-    apply Mem.bounds_alloc with (b':=b) in J; auto.
-    destruct (eq_block b mb); subst.
-      destruct J4 as [J4 _].
-      assert (J':=J2).
-      apply Mem.nextblock_alloc in J2; subst.
-      apply Mem.alloc_result in J'; subst.
-      contradict G; zauto.
-
-      rewrite J. auto.
-Qed.
-
-Lemma store_preserves_wf_global_ptr : forall S TD Mem0 gl gvp t gv align Mem',
-  mstore TD Mem0 gvp t gv align = Some Mem' ->
-  wf_global_ptr S TD Mem0 gl ->
-  wf_global_ptr S TD Mem' gl.
-Proof.
-  intros.
-  apply store_inv in H.
-  destruct H as [b [ofs [c [v0 [J1 [J2 [J3 J4]]]]]]].
-  intros x gv0 typ0 Hlk Hwfc.
-  eapply H0 in Hwfc; eauto.
-  destruct Hwfc as [b' [sz0 [J5 [J6 [J7 J8]]]]].
-  eapply store_preserves_temoporal_prop in J8; eauto.
-  exists b'. exists sz0.
-  repeat (split; auto).
-    erewrite Mem.bounds_store; eauto.
-Qed.
-
-Lemma callExternalFunction_preserves_wf_global_ptr : forall Mem0 fid gvs oresult
-    Mem' S TD gl,
-  callExternalFunction Mem0 fid gvs = Some (oresult, Mem') ->
-  wf_global_ptr S TD Mem0 gl ->
-  wf_global_ptr S TD Mem' gl.
-Proof.
-  intros.
-  intros x gv0 typ0 Hlk Hwfc.
-  eapply H0 in Hwfc; eauto.
-  destruct Hwfc as [b [sz0 [J5 [J6 [J7 J8]]]]].
-  exists b. exists sz0. 
-  repeat (split; eauto using callExternalFunction_temporal_prop).
-    erewrite <- callExternalFunction_mem_bounds; eauto.
-Qed.
-
 (********************************************)
 (* wf_rmetadata *)
-
-Lemma free_preserves_wf_rmetadata : forall TD (Mem0 Mem' : mem) gv 
-  (H0 : free TD Mem0 gv = ret Mem') rm (Hwfr : wf_rmetadata TD Mem0 rm),
-  wf_rmetadata TD Mem' rm.
-Proof.
-  intros. 
-  apply free_inv in H0. 
-  destruct H0 as [blk [ofs [hi [lo [J1 [J2 [J3 J4]]]]]]].
-  intros i1 gvb gve J.
-  apply Hwfr in J.   
-  eapply free_preserves_wf_data; eauto.
-Qed.
-
-Lemma free_allocas_preserves_wf_rmetadata : forall als TD M M' rm,
-  free_allocas TD M als = Some M' ->
-  wf_rmetadata TD M rm ->
-  wf_rmetadata TD M' rm.
-Proof.
-  induction als; simpl; intros TD M M' rm Hfree Hwfr.
-    inv Hfree. auto.
-
-    remember (free TD M (blk2GV TD a)) as R.
-    destruct R; inv Hfree.
-    eapply IHals; eauto.
-    eapply free_preserves_wf_rmetadata in Hwfr; eauto.
-Qed.
-
-Lemma malloc_preserves_wf_rmetadata : forall (TD : TargetData) rm gn align0
-  (Mem0 Mem' : mem) (tsz : sz) (mb : mblock)
-  (H1 : malloc TD Mem0 tsz gn align0 = ret (Mem', mb))
-  (Hwfr : wf_rmetadata TD Mem0 rm),
-  wf_rmetadata TD Mem' rm.
-Proof.
-  intros. 
-  apply malloc_inv in H1. 
-  destruct H1 as [n [J1 [J2 J3]]].
-  intros i1 gvb gve J.
-  apply Hwfr in J.   
-  eapply alloc_preserves_wf_data; eauto.
-Qed.
-  
-Lemma malloc_extends_wf_rmetadata : forall
-  (TD : TargetData)
-  (rm : AssocList metadata)
-  (lc : GVsMap)
-  (id0 : atom)
-  (gn : GenericValue)
-  (align0 : align)
-  (Mem0 : mem)
-  (Mem' : mem)
-  (tsz : sz)
-  (mb : mblock)
-  (lc' : GVsMap)
-  (rm' : rmetadata)
-  (n : Z) t
-  (H1 : malloc TD Mem0 tsz gn align0 = ret (Mem', mb))
-  (H2 : GV2int TD Size.ThirtyTwo gn = ret n)
-  (H3 : prop_reg_metadata lc rm id0 ($ (blk2GV TD mb) # typ_pointer t $)
-         {| md_base := base2GV TD mb; md_bound := bound2GV TD mb tsz n |} =
-       (lc', rm'))
-  (Hwfr : wf_rmetadata TD Mem0 rm),
-  wf_rmetadata TD Mem' rm'.
-Proof.
-  intros.
-  invert_prop_reg_metadata. clear H3.
-  unfold malloc in H1.
-  rewrite H2 in H1.
-  destruct (zle 0 (Size.to_Z tsz * n)); try solve [inversion H1].
-  remember (Mem.alloc Mem0 0 (Size.to_Z tsz * n)) as R.
-  inversion H1. clear H1. subst.
-  clear H2.
-  intros i0 gvb gve J.
-  destruct (@id_dec id0 i0); subst.
-  SCase "id0=i0".
-      rewrite lookupAL_updateAddAL_eq in J.
-      inversion J; subst. clear J.
-      unfold wf_data.
-      rewrite GV2ptr_base2GV. 
-      rewrite GV2ptr_bound2GV. 
-      destruct (zeq mb mb) as [J | J]; try solve [contradict J; auto].
-      split.
-        assert (H4':=H0).
-        apply Mem.alloc_result in H0.
-        apply Mem.nextblock_alloc in H4'.
-        rewrite H0. rewrite H4'. zauto.
-
-        intros Hwfb ofs J1. 
-        apply Mem.valid_access_alloc_same with (ofs:=ofs)(chunk:=AST.Mint 7) 
-          in H0.
-          destruct H0 as [J2 J3].
-          unfold Mem.range_perm in J2.
-          apply Mem.perm_implies with (p1:=Freeable); auto with mem.
-          apply J2.
-          simpl. clear.
-          assert (J:=@bytesize_chunk_pos 7).
-          zauto.
-
-          rewrite Int.signed_repr in J1; zauto. clear.
-          assert (J1:=@Int.min_signed_neg 31).          
-          assert (J2:=@Int.max_signed_pos 31).          
-          zauto.
-
-          simpl. rewrite bytesize_chunk_7_eq_1. 
-          destruct J1 as [_ J1].
-          unfold Int.signed in J1.
-          unfold Int.unsigned in J1.
-          simpl in J1.
-          clear - J1 z.
-          assert (J:=@Int.modulus_pos 31).
-          assert ((Size.to_Z tsz * n) mod Int.modulus 31 <= (Size.to_Z tsz * n)) 
-            as LE.
-            apply Zmod_le; zauto.
-          destruct (zlt ((Size.to_Z tsz * n) mod Int.modulus 31) 
-            (Int.half_modulus 31)); zeauto.
-
-          simpl. rewrite bytesize_chunk_7_eq_1. zauto.
-
-  SCase "id0<>i0".
-      rewrite <- lookupAL_updateAddAL_neq in J; auto.
-      assert (J':=@Hwfr i0 gvb gve J). clear Hwfr.    
-      eapply alloc_preserves_wf_data; eauto.
-Qed.
 
 Lemma returnUpdateLocals__wf_rmetadata : forall los nts Result lc rm gl c' lc' 
     rm' Mem0 Mem' als lc'' rm'' S Ps f rt
@@ -1091,7 +503,7 @@ Proof.
     destruct R3 as [[md ?]|]; try solve [inv H1; auto].
     destruct c'; try solve [inv H1; auto].
     destruct n; try solve [inv H1; auto].
-    unfold isReturnPointerTypB, isPointerTypB in H1.
+    unfold SBopsem.isReturnPointerTypB, isPointerTypB in H1.
     destruct t; try solve [inv H1; auto].
     destruct t; inv H1; auto.
       intros x gvb gve Hlk.
@@ -1106,7 +518,7 @@ Proof.
 
     destruct c'; try solve [inv H1; auto].
     destruct n; try solve [inv H1; auto].
-    unfold isReturnPointerTypB, isPointerTypB in H1.
+    unfold SBopsem.isReturnPointerTypB, isPointerTypB in H1.
     destruct t; try solve [inv H1; auto].
     destruct t; inv H1; auto.
       intros x gvb gve Hlk.
@@ -1235,38 +647,6 @@ Proof.
     apply NoDup_inv in HBinF. destruct HBinF; auto.
 Qed.
 
-Lemma get_mem_metadata__wf_rmetadata : forall los nts Mem0 rm gvp id0 MM,
-  wf_mmetadata (los, nts) Mem0 MM ->
-  wf_rmetadata (los, nts) Mem0 rm ->
-  wf_rmetadata (los, nts) Mem0 
-    (updateAddAL metadata rm id0 (get_mem_metadata (los, nts) MM gvp)).
-Proof.
-  intros.
-  intros i0 gvb gve J.
-  destruct (@id_dec id0 i0); subst.
-    rewrite lookupAL_updateAddAL_eq in J.
-    inversion J; subst.
-    eapply wf_mmetadata__get_mem_metadata in H2; eauto.
-
-    rewrite <- lookupAL_updateAddAL_neq in J; auto. eauto.
-Qed.
-
-Lemma store_preserves_wf_rmetadata : forall TD Mem0 gvp t gv align0 Mem' rm, 
-  mstore TD Mem0 gvp t gv align0 = ret Mem' ->
-  wf_rmetadata TD Mem0 rm -> 
-  wf_rmetadata TD Mem' rm.
-Proof. 
-  intros TD Mem0 gvp t gv align0 Mem' rm H3 Hwfr.
-  unfold mstore in H3.
-  destruct (GV2ptr TD (getPointerSize TD) gvp); try solve [inversion H3].
-  destruct v; try solve [inversion H3].
-  destruct (typ2memory_chunk t); try solve [inversion H3].
-  destruct (GV2val TD gv); try solve [inversion H3].
-  intros i1 gvb gve J.
-  apply Hwfr in J. clear Hwfr.
-  eapply wf_data__store__wf_data; eauto.
-Qed.
-
 Lemma prop_metadata_preserves_wf_rmetadata : forall los nts Mem0 rm md gl S Ps
     f t id0 vp
   (H : get_reg_metadata (los, nts) gl rm vp = ret md)
@@ -1284,28 +664,6 @@ Proof.
 
     rewrite <- lookupAL_updateAddAL_neq in J0; auto.
     apply Hwfr in J0; auto.
-Qed.
-
-Lemma adding_null_preserves_wf_rmetadata : forall TD Mem0 rm id0,
-  wf_rmetadata TD Mem0 rm ->
-  wf_rmetadata TD Mem0
-    (updateAddAL metadata rm id0 {| md_base := null; md_bound := null |}).
-Proof.
-  intros TD Mem0 rm id0 Hwfr.
-  intros i0 gvb gve J.
-  destruct (@id_dec id0 i0); subst.
-    rewrite lookupAL_updateAddAL_eq in J.
-    inversion J; subst. clear J.
-    unfold wf_data.
-    simpl.
-    split.
-      apply nullptr_lt_nextblock.
-  
-      intros Htmp ofs J.
-      contradict J; zauto.
-  
-    rewrite <- lookupAL_updateAddAL_neq in J; auto.
-    apply Hwfr in J; auto.
 Qed.
 
 Lemma params2GVs__wf_rmetadata : forall S los nts Ps f M rm lc gl ps ogvs
@@ -1426,67 +784,91 @@ Proof.
     intros x bv gv J. inv J.
 Qed.
 
-Lemma callExternalFunction_preserves_wf_rmetadata : forall Mem0 fid gvs oresult
-    Mem' rm TD,
-  callExternalFunction Mem0 fid gvs = Some (oresult, Mem') ->
-  wf_rmetadata TD Mem0 rm ->
-  wf_rmetadata TD Mem' rm.
+Lemma malloc_extends_wf_rmetadata : forall
+  (TD : TargetData)
+  (rm : AssocList metadata)
+  (lc : GVsMap)
+  (id0 : atom)
+  (gn : GenericValue)
+  (align0 : align)
+  (Mem0 : mem)
+  (Mem' : mem)
+  (tsz : sz)
+  (mb : mblock)
+  (lc' : GVsMap)
+  (rm' : rmetadata)
+  (n : Z) t
+  (H1 : malloc TD Mem0 tsz gn align0 = ret (Mem', mb))
+  (H2 : GV2int TD Size.ThirtyTwo gn = ret n)
+  (H3 : prop_reg_metadata lc rm id0 ($ (blk2GV TD mb) # typ_pointer t $)
+         {| md_base := base2GV TD mb; md_bound := bound2GV TD mb tsz n |} =
+       (lc', rm'))
+  (Hwfr : wf_rmetadata TD Mem0 rm),
+  wf_rmetadata TD Mem' rm'.
 Proof.
-  intros Mem0 fid gvs oresult Mem' rm TD Hcall Hwfr.
-  intros x bv ev Hlk.
-  apply Hwfr in Hlk.
-  unfold wf_data in *.
-  destruct (GV2ptr TD (getPointerSize TD) bv); try solve [inv Hlk].
-  destruct v; try solve [inv Hlk].
-  destruct (GV2ptr TD (getPointerSize TD) ev); try solve [inv Hlk].
-  destruct v; try solve [inv Hlk].
-  destruct (zeq b b0); subst; auto.
-    eauto using callExternalFunction_temporal_prop.
+  intros.
+  invert_prop_reg_metadata. clear H3.
+  unfold malloc in H1.
+  rewrite H2 in H1.
+  destruct (zle 0 (Size.to_Z tsz * n)); try solve [inversion H1].
+  remember (Mem.alloc Mem0 0 (Size.to_Z tsz * n)) as R.
+  inversion H1. clear H1. subst.
+  clear H2.
+  intros i0 gvb gve J.
+  destruct (@id_dec id0 i0); subst.
+  SCase "id0=i0".
+      rewrite lookupAL_updateAddAL_eq in J.
+      inversion J; subst. clear J.
+      unfold wf_data.
+      rewrite GV2ptr_base2GV. 
+      rewrite GV2ptr_bound2GV. 
+      destruct (zeq mb mb) as [J | J]; try solve [contradict J; auto].
+      split.
+        assert (H4':=H0).
+        apply Mem.alloc_result in H0.
+        apply Mem.nextblock_alloc in H4'.
+        rewrite H0. rewrite H4'. zauto.
+
+        intros Hwfb ofs J1. 
+        apply Mem.valid_access_alloc_same with (ofs:=ofs)(chunk:=AST.Mint 7) 
+          in H0.
+          destruct H0 as [J2 J3].
+          unfold Mem.range_perm in J2.
+          apply Mem.perm_implies with (p1:=Freeable); auto with mem.
+          apply J2.
+          simpl. clear.
+          assert (J:=@bytesize_chunk_pos 7).
+          zauto.
+
+          rewrite Int.signed_repr in J1; zauto. clear.
+          assert (J1:=@Int.min_signed_neg 31).          
+          assert (J2:=@Int.max_signed_pos 31).          
+          zauto.
+
+          simpl. rewrite bytesize_chunk_7_eq_1. 
+          destruct J1 as [_ J1].
+          unfold Int.signed in J1.
+          unfold Int.unsigned in J1.
+          simpl in J1.
+          clear - J1 z.
+          assert (J:=@Int.modulus_pos 31).
+          assert ((Size.to_Z tsz * n) mod Int.modulus 31 <= (Size.to_Z tsz * n)) 
+            as LE.
+            apply Zmod_le; zauto.
+          destruct (zlt ((Size.to_Z tsz * n) mod Int.modulus 31) 
+            (Int.half_modulus 31)); zeauto.
+
+          simpl. rewrite bytesize_chunk_7_eq_1. zauto.
+
+  SCase "id0<>i0".
+      rewrite <- lookupAL_updateAddAL_neq in J; auto.
+      assert (J':=@Hwfr i0 gvb gve J). clear Hwfr.    
+      eapply alloc_preserves_wf_data; eauto.
 Qed.
 
 (********************************************)
 (* wf_mmetadata *)
 
-Lemma free_preserves_wf_mmetadata : forall TD (Mem0 Mem' : mem) gv
-  (H0 : free TD Mem0 gv = ret Mem') MM (Hwfm : wf_mmetadata TD Mem0 MM),
-  wf_mmetadata TD Mem' MM.
-Proof.
-  intros. 
-  apply free_inv in H0. 
-  destruct H0 as [blk [ofs [hi [lo [J1 [J2 [J3 J4]]]]]]].
-  intros b1 ofs' gvb gve J.
-  assert (J':=@Hwfm b1 ofs' gvb gve J).
-  eapply free_preserves_wf_data; eauto.
-Qed.
-
-Lemma free_allocas_preserves_wf_mmetadata : forall als TD M M' MM,
-  free_allocas TD M als = Some M' ->
-  wf_mmetadata TD M MM ->
-  wf_mmetadata TD M' MM.
-Proof.
-  induction als; simpl; intros TD M M' MM Hfree Hwfr.
-    inv Hfree. auto.
-
-    remember (free TD M (blk2GV TD a)) as R.
-    destruct R; inv Hfree.
-    eapply IHals; eauto.
-    eapply free_preserves_wf_mmetadata in Hwfr; eauto.
-Qed.
-
-Lemma malloc_preserves_wf_mmetadata : forall (TD : TargetData) MM gn align0
-  (Mem0 Mem' : mem) (tsz : sz) (mb : mblock)
-  (H1 : malloc TD Mem0 tsz gn align0 = ret (Mem', mb))
-  (Hwfm : wf_mmetadata TD Mem0 MM),
-  wf_mmetadata TD Mem' MM.
-Proof.
-  intros. 
-  apply malloc_inv in H1. 
-  destruct H1 as [n [J1 [J2 J3]]].
-  intros b ofs gvb gve J.
-  assert (J':=@Hwfm b ofs gvb gve J).
-  eapply alloc_preserves_wf_data; eauto.
-Qed.
-  
 Lemma malloc_extends_wf_mmetadata : forall
   (TD : TargetData)
   (lc : GVsMap)
@@ -1520,205 +902,6 @@ Proof.
   assert (J':=@Hwfm b ofs gvb gve J). clear Hwfm.
   eapply alloc_preserves_wf_data; eauto.
 Qed.
-
-Lemma store_nptr_preserves_wf_mmetadata : forall TD Mem0 gvp t gv align0 Mem' MM,
-  mstore TD Mem0 gvp t gv align0 = ret Mem' ->
-  wf_mmetadata TD Mem0 MM -> 
-  wf_mmetadata TD Mem' MM.
-Proof. 
-  intros TD Mem0 gvp t gv align0 Mem' rm H3 Hwfm.
-  unfold mstore in H3.
-  destruct (GV2ptr TD (getPointerSize TD) gvp); try solve [inversion H3].
-  destruct v; try solve [inversion H3].
-  destruct (typ2memory_chunk t); try solve [inversion H3].
-  destruct (GV2val TD gv); try solve [inversion H3].
-  intros b0 ofs gvb gve J.
-  apply Hwfm in J. clear Hwfm.
-  eapply wf_data__store__wf_data; eauto.
-Qed.
-
-Lemma store_ptr_preserves_wf_mmetadata : forall los nts Mem0 rm MM md' gl S
-    gvp gv align0 Mem' Ps f v t
-  (Hwfg' : wf_global_ptr S (los, nts) Mem0 gl)
-  (Hwfm1' : wf_rmetadata (los, nts) Mem0 rm)
-  (H3 : mstore (los, nts) Mem0 gvp t gv align0 = ret Mem')
-  (H5 : get_reg_metadata (los, nts) gl rm v = ret md')
-  (Hwfv : wf_value S (module_intro los nts Ps) f v t)
-  (Hwfm : wf_mmetadata (los, nts) Mem0 MM),
-  wf_mmetadata (los, nts) Mem' (set_mem_metadata (los, nts) MM gvp md').
-Proof.
-  intros.
-  unfold mstore in H3.
-  destruct (GV2ptr (los,nts) (getPointerSize (los,nts)) gvp); 
-    try solve [inversion H3].
-  destruct v0; try solve [inversion H3].
-  destruct (typ2memory_chunk t); try solve [inversion H3].
-  destruct (GV2val (los,nts) gv); try solve [inversion H3].
-  intros b0 ofs gvb gve J. 
-    subst.
-    unfold set_mem_metadata in J.
-    destruct (GV2ptr (los,nts) (getPointerSize (los,nts)) gvp); 
-      try solve [eauto using wf_mmetadata__store__wf_data].
-    destruct v1; try solve [eauto using wf_mmetadata__store__wf_data].
-    destruct (zeq b0 b1); subst; 
-       simpl in J; eauto using wf_mmetadata__store__wf_data.
-    destruct (Int.eq_dec 31 i1 ofs); subst; 
-       simpl in J; eauto using wf_mmetadata__store__wf_data.
-  
-       inversion J; subst. clear J.
-       eapply wf_rmetadata__get_reg_metadata with (Mem0:=Mem0) in H5; eauto.
-         eapply wf_data__store__wf_data; eauto.
-Qed.
-
-Lemma callExternalFunction_preserves_wf_mmetadata : forall Mem0 fid gvs oresult
-    Mem' TD MM,
-  callExternalFunction Mem0 fid gvs = Some (oresult, Mem') ->
-  wf_mmetadata TD Mem0 MM ->
-  wf_mmetadata TD Mem' MM.
-Proof.
-  intros Mem0 fid gvs oresult Mem' TD MM Hcall Hwfm.
-  intros b ofs bv ev Hlk.
-  apply Hwfm in Hlk.
-  unfold wf_data in *.
-  destruct (GV2ptr TD (getPointerSize TD) bv); try solve [inv Hlk].
-  destruct v; try solve [inv Hlk].
-  destruct (GV2ptr TD (getPointerSize TD) ev); try solve [inv Hlk].
-  destruct v; try solve [inv Hlk].
-  destruct (zeq b0 b1); subst; auto.
-    eauto using callExternalFunction_temporal_prop.
-Qed.
-
-(********************************************)
-(* assert_mptr *)
-
-Lemma typ2memory_chunk__le__getTypeAllocSize : forall sys t c s TD,
-  wf_typ sys t ->
-  (forall a b o, 
-    getTypeSizeInBits_and_Alignment TD o t = Some (a,b) ->
-    (b > 0)%nat) ->
-  typ2memory_chunk t = Some c ->
-  Some s = getTypeAllocSize TD t ->
-  size_chunk c <= Size.to_Z s.
-Proof.
-  intros sys t c s TD Hwft Hwfa H1 H2.
-  unfold getTypeAllocSize, getTypeStoreSize, getTypeSizeInBits, 
-         getTypeSizeInBits_and_Alignment in H2.
-  assert (Z_of_nat 0 = 0) as EQ0. simpl. auto.
-  destruct TD.
-  destruct t; inv H1; inv H2;
-    simpl; unfold bytesize_chunk, Size.to_nat, RoundUpAlignment, Size.to_Z.
-    assert (ZRdiv (Z_of_nat s0) 8 >= 0) as J.
-      apply ZRdiv_prop2; zauto.
-    assert (Z_of_nat 0 = 0) as EQ. simpl. auto.
-    assert (Z_of_nat (getIntAlignmentInfo l0 s0 true) > 0) as GT.
-      rewrite <- EQ0.
-      apply inj_gt.
-      eapply Hwfa; simpl; eauto.
-    assert (ZRdiv (Z_of_nat (S (s0 - 1))) 8 <= ZRdiv (Z_of_nat s0) 8) as J2.  
-      unfold ZRdiv.
-      apply ZRdiv_prop7.
-        apply inj_le.
-          inv Hwft. unfold Size.gt in H1. omega.
-        apply Z_of_S_gt_O.
-    assert (J':=@roundup_is_correct (ZRdiv (Z_of_nat s0) 8)
-      (Z_of_nat (getIntAlignmentInfo l0 s0 true)) GT). 
-    rewrite nat_of_Z_eq.
-      rewrite nat_of_Z_eq; auto.
-        zauto.
-      rewrite nat_of_Z_eq; auto.
-        zauto.
-
-    destruct f; inv H0; inv H1; simpl; unfold RoundUpAlignment.
-      assert (Z_of_nat (getFloatAlignmentInfo l0 32 true) > 0) as GT.
-        rewrite <- EQ0.
-        apply inj_gt.
-        eapply Hwfa; simpl; eauto.
-      rewrite <- Zpos_eq_Z_of_nat_o_nat_of_P.
-      assert (J:=@roundup_is_correct 4 (Z_of_nat 
-        (getFloatAlignmentInfo l0 32 true)) GT).
-      rewrite nat_of_Z_eq; zauto. 
-
-      assert (Z_of_nat (getFloatAlignmentInfo l0 64 true) > 0) as GT.
-        rewrite <- EQ0.
-        apply inj_gt.
-        eapply Hwfa; simpl; eauto.
-      rewrite <- Zpos_eq_Z_of_nat_o_nat_of_P.
-      assert (J:=@roundup_is_correct 8 (Z_of_nat 
-        (getFloatAlignmentInfo l0 64 true)) GT).
-      rewrite nat_of_Z_eq; zauto. 
-
-    assert (Z_of_nat (getPointerAlignmentInfo l0 true) > 0) as GT.
-      rewrite <- EQ0.
-      apply inj_gt.
-      eapply Hwfa; simpl; eauto.
-    rewrite <- Zpos_eq_Z_of_nat_o_nat_of_P.
-    assert (J:=@roundup_is_correct 4 (Z_of_nat 
-      (getPointerAlignmentInfo l0 true)) GT).
-    assert (ZRdiv (Z_of_nat 32) 8 = 4) as EQ.
-      unfold ZRdiv. simpl. zauto.
-    rewrite EQ. clear EQ.
-    rewrite nat_of_Z_max.
-    rewrite Zmax_left; zauto.
-Qed.
-
-Lemma assert_mptr__valid_access : forall S md los nts Ps Mem gl rm MM t g b ofs
-    c f v tv,
-  wf_metadata (los, nts) Mem rm MM ->
-  wf_global_ptr S (los, nts) Mem gl ->
-  wf_value S (module_intro los nts Ps) f v tv ->
-  Some md = get_reg_metadata (los, nts) gl rm v ->
-  wf_typ S t ->
-  (forall a b o, 
-    getTypeSizeInBits_and_Alignment (los, nts) o t = Some (a,b) ->
-    (b > 0)%nat) ->
-  assert_mptr (los, nts) t g md ->
-  GV2ptr (los, nts) (getPointerSize (los, nts)) g = ret Values.Vptr b ofs ->
-  typ2memory_chunk t = ret c ->
-  (align_chunk c | Int.signed 31 ofs) ->
-  blk_temporal_safe Mem b ->
-  Mem.valid_access Mem c b (Int.signed 31 ofs) Writable.
-Proof.
-  intros S md los nts Ps Mem gl rm MM t g b ofs c f v tv Hwf Hwfg Hwfv Heqmd
-    Hwft Hwfa J R3 R4 R5 Htmp.
-  unfold Mem.valid_access.
-  split; auto.
-    unfold assert_mptr in J.
-    rewrite R3 in J.
-    symmetry in Heqmd.  
-    destruct md.
-    destruct Hwf as [Hwfr Hwfm].
-    eapply wf_rmetadata__get_reg_metadata in Heqmd; eauto.
-    unfold wf_data in Heqmd.
-    unfold layouts, namedts in J.
-    destruct (GV2ptr (@pair (list layout) (list namedt) los nts)
-              (getPointerSize (@pair (list layout) (list namedt) los nts))
-              md_base0);
-      try solve [inversion Heqmd].
-    destruct v0; try solve [inversion Heqmd].
-    destruct (GV2ptr (@pair (list layout) (list namedt) los nts)
-              (getPointerSize (@pair (list layout) (list namedt) los nts))
-              md_bound0);
-      try solve [inversion Heqmd].
-    destruct v0; try solve [inversion Heqmd].
-    destruct (zeq b0 b1); subst; try solve [inversion Heqmd].
-    remember (getTypeAllocSize (@pair (list layout) (list namedt) los nts) t)
-      as R6.
-    destruct R6; try solve [inversion J].
-    simpl in J.
-    intros z Jz.
-    bdestruct4 J as J1 J4 J2 J3.
-    destruct (zeq b b1); subst; try solve [inversion J1].
-    apply Heqmd; auto.
-    clear - J2 J3 Jz HeqR6 R4 Hwfa Hwft.
-    assert (size_chunk c <= Size.to_Z s) as J4.
-      eapply typ2memory_chunk__le__getTypeAllocSize; eauto.
-    destruct (zle (Int.signed 31 i0) (Int.signed 31 ofs)); 
-      simpl in J2; inversion J2.
-    destruct (zle (Int.signed 31 ofs + Size.to_Z s) (Int.signed 31 i1)); 
-      simpl in J3; inversion J3.
-    zeauto.
-Qed.
-
 
 (*****************************)
 (*
